Added a more generic iterator "iterato" ("o" for "ordered"), analogous to "iterate" and collapsing to it in the usual universal commuting case, and then its instantiations to two slightly different iterated operations on groups, "group_product" (a product in order, an order given explicitly as an argument) and "group_sum" (using an arbitrary wellorder, intended for cases where it doesn't matter such as Abelian groups or more specific settings in general groups). Also added a miscellany of other theorems, some about machine words, a few arithmetic/divisibility ones. New definitions:
        iterato
        group_product
        group_sum

and theorems:

        ABELIAN_GROUP_PRODUCT_CLAUSES
        ABELIAN_GROUP_SUM_CLAUSES
        BITVAL_POS
        CONG_DIV2
        CONG_DIV_COPRIME
        EMPTY_NUMSEG
        EQ_BITVAL
        EXISTS_SWAP_FUN_THM
        GROUP_COMMUTES_MUL
        GROUP_COMMUTES_PRODUCT
        GROUP_COMMUTES_SUM
        GROUP_PRODUCT
        GROUP_PRODUCT_CLAUSES
        GROUP_PRODUCT_CLAUSES_COMMUTING
        GROUP_PRODUCT_CLAUSES_EXISTS
        GROUP_PRODUCT_CLAUSES_LEFT
        GROUP_PRODUCT_CLAUSES_NUMSEG
        GROUP_PRODUCT_CLAUSES_RIGHT
        GROUP_PRODUCT_CLOSED
        GROUP_PRODUCT_EQ
        GROUP_PRODUCT_EXPAND_CASES
        GROUP_PRODUCT_MUL
        GROUP_PRODUCT_RESTRICT
        GROUP_PRODUCT_SING
        GROUP_PRODUCT_SUPPORT
        GROUP_PRODUCT_UNION
        GROUP_SUM
        GROUP_SUM_CLAUSES_COMMUTING
        GROUP_SUM_CLAUSES_EXISTS
        GROUP_SUM_CLOSED
        GROUP_SUM_EQ
        GROUP_SUM_EXPAND_CASES
        GROUP_SUM_MUL
        GROUP_SUM_RESTRICT
        GROUP_SUM_SING
        GROUP_SUM_SUPPORT
        INT_CONG_DIV
        INT_CONG_DIV2
        INT_CONG_DIV_COPRIME
        INT_EQ_BITVAL
        INT_LE_BITVAL
        INT_VAL_WORD_NOT
        ITERATO_CLAUSES
        ITERATO_CLAUSES_EXISTS
        ITERATO_CLAUSES_GEN
        ITERATO_CLAUSES_NUMSEG_LEFT
        ITERATO_CLOSED
        ITERATO_EQ
        ITERATO_EXPAND_CASES
        ITERATO_INDUCT
        ITERATO_ITERATE
        ITERATO_SUPPORT
        LE_BITVAL
        REAL_BITVAL_NOT
        REAL_EQ_BITVAL
        REAL_LE_BITVAL
        REAL_OF_NUM_CLAUSES
        REAL_VAL_WORD_NOT
        VAL_EQ_MAX_MASK
        VAL_MOD_2
        WORD_AND_1_BITVAL
        WORD_NEG_AND_MASK

Library/grouptheory.ml
@@ -351,6 +351,16 @@ let GROUP_COMMUTES_INV_EQ = prove
              group_mul G x y = group_mul G y x)`,
   MESON_TAC[GROUP_COMMUTES_INV; GROUP_INV_INV; GROUP_INV]);;
 
+let GROUP_COMMUTES_MUL = prove
+ (`!G x y z:A.
+        x IN group_carrier G /\
+        y IN group_carrier G /\
+        z IN group_carrier G /\
+        group_mul G x z = group_mul G z x /\
+        group_mul G y z = group_mul G z y
+        ==> group_mul G (group_mul G x y) z = group_mul G z (group_mul G x y)`,
+  MESON_TAC[GROUP_MUL; GROUP_MUL_ASSOC]);;
+
 let FORALL_IN_GROUP_CARRIER_INV = prove
  (`!(P:A->bool) G.
         (!x. x IN group_carrier G ==> P(group_inv G x)) <=>
@@ -1044,6 +1054,496 @@ let GROUP_RULE =
     let th4 = GENL avs th3 in
     let bvs = frees(concl th4) in
     GENL (sort (<) bvs) th4;;
+
+(* ------------------------------------------------------------------------- *)
+(* Iterated operation on groups, the first one being in a specific           *)
+(* order given as an argument, the latter picking some arbitrary             *)
+(* wellorder, usually with the expectation that it will be immaterial.       *)
+(* ------------------------------------------------------------------------- *)
+
+let group_product = new_definition
+ `group_product (G:A group) =
+        iterato (group_carrier G) (group_id G) (group_mul G)`;;
+
+let group_sum = new_definition
+ `group_sum (G:A group) =
+        group_product G (@l. woset l /\ fld l = (:K))`;;
+
+let GROUP_PRODUCT_EQ = prove
+ (`!G (<<=) k (f:K->A) g.
+        (!i. i IN k ==> f i = g i)
+        ==> group_product G (<<=) k f = group_product G (<<=) k g`,
+  REWRITE_TAC[group_product; ITERATO_EQ]);;
+
+let GROUP_SUM_EQ = prove
+ (`!G k (f:K->A) g.
+        (!i. i IN k ==> f i = g i) ==> group_sum G k f = group_sum G k g`,
+  REWRITE_TAC[group_sum; GROUP_PRODUCT_EQ]);;
+
+let GROUP_PRODUCT_CLOSED = prove
+ (`!P G (<<=) k (f:K->A).
+       P(group_id G) /\
+       (!x y. x IN group_carrier G /\ y IN group_carrier G /\
+              P x /\ P y
+              ==> P(group_mul G x y)) /\
+       (!i. i IN k /\ f i IN group_carrier G /\ ~(f i = group_id G) ==> P(f i))
+       ==> P(group_product G (<<=) k f)`,
+  REPEAT STRIP_TAC THEN REWRITE_TAC[group_product] THEN
+  MP_TAC(ISPECL
+   [`group_carrier G:A->bool`; `group_id G:A`; `group_mul G:A->A->A`;
+    `(<<=):K->K->bool`; `k:K->bool`; `f:K->A`;
+    `\x:A. x IN group_carrier G /\ P x`]
+   ITERATO_CLOSED) THEN
+  ASM_SIMP_TAC[GROUP_ID; GROUP_MUL]);;
+
+let GROUP_SUM_CLOSED = prove
+ (`!P G k (f:K->A).
+       P(group_id G) /\
+       (!x y. x IN group_carrier G /\ y IN group_carrier G /\
+              P x /\ P y
+              ==> P(group_mul G x y)) /\
+       (!i. i IN k /\ f i IN group_carrier G /\ ~(f i = group_id G) ==> P(f i))
+       ==> P(group_sum G k f)`,
+  REWRITE_TAC[group_sum; GROUP_PRODUCT_CLOSED]);;
+
+let GROUP_PRODUCT = prove
+ (`!G (<<=) k (f:K->A). group_product G (<<=) k f IN group_carrier G`,
+  REPEAT STRIP_TAC THEN MATCH_MP_TAC (REWRITE_RULE[]
+   (ISPEC `\x:A. x IN group_carrier G` GROUP_PRODUCT_CLOSED)) THEN
+  SIMP_TAC[GROUP_ID; GROUP_MUL]);;
+
+let GROUP_SUM = prove
+ (`!G k (f:K->A). group_sum G k f IN group_carrier G`,
+  REWRITE_TAC[group_sum; GROUP_PRODUCT]);;
+
+let GROUP_PRODUCT_SUPPORT = prove
+ (`!G (<<=) k (f:K->A).
+        group_product G (<<=) {i | i IN k /\ ~(f i = group_id G)} f =
+        group_product G (<<=) k f`,
+  REPEAT GEN_TAC THEN REWRITE_TAC[group_product] THEN
+  ONCE_REWRITE_TAC[GSYM ITERATO_SUPPORT] THEN
+  AP_THM_TAC THEN AP_TERM_TAC THEN SET_TAC[]);;
+
+let GROUP_SUM_SUPPORT = prove
+ (`!G k (f:K->A).
+      group_sum G {i | i IN k /\ ~(f i = group_id G)} f =
+      group_sum G k f`,
+  REWRITE_TAC[group_sum; GROUP_PRODUCT_SUPPORT]);;
+
+let GROUP_PRODUCT_RESTRICT = prove
+ (`!G (<<=) k (f:K->A).
+        group_product G (<<=) {i | i IN k /\ f i IN group_carrier G} f =
+        group_product G (<<=) k f`,
+  REPEAT GEN_TAC THEN REWRITE_TAC[group_product] THEN
+  ONCE_REWRITE_TAC[GSYM ITERATO_SUPPORT] THEN
+  AP_THM_TAC THEN AP_TERM_TAC THEN SET_TAC[]);;
+
+let GROUP_SUM_RESTRICT = prove
+ (`!G k (f:K->A).
+        group_sum G {i | i IN k /\ f i IN group_carrier G} f =
+        group_sum G k f`,
+  REWRITE_TAC[group_sum; GROUP_PRODUCT_RESTRICT]);;
+
+let GROUP_PRODUCT_EXPAND_CASES = prove
+ (`!G (<<=) k (f:K->A).
+        group_product G (<<=) k f =
+        if FINITE {i | i IN k /\ f i IN group_carrier G DIFF {group_id G}}
+        then group_product G (<<=)
+              {i | i IN k /\ f i IN group_carrier G DIFF {group_id G}} f
+        else group_id G`,
+  REPEAT GEN_TAC THEN REWRITE_TAC[group_product] THEN
+  MATCH_ACCEPT_TAC ITERATO_EXPAND_CASES);;
+
+let GROUP_SUM_EXPAND_CASES = prove
+ (`!G k (f:K->A).
+        group_sum G k f =
+        if FINITE {i | i IN k /\ f i IN group_carrier G DIFF {group_id G}}
+        then group_sum G
+              {i | i IN k /\ f i IN group_carrier G DIFF {group_id G}} f
+        else group_id G`,
+  REPEAT GEN_TAC THEN REWRITE_TAC[group_sum] THEN
+  MATCH_ACCEPT_TAC GROUP_PRODUCT_EXPAND_CASES);;
+
+let GROUP_PRODUCT_CLAUSES = prove
+ (`!G (<<=) (f:K->A).
+      group_product G (<<=) {} f = group_id G /\
+      (!i k. FINITE {j | j IN k /\ f j IN group_carrier G DIFF {group_id G}} /\
+             (!j. j IN k ==> i <<= j /\ ~(j <<= i))
+             ==> group_product G (<<=) (i INSERT k) f =
+                   if f i IN group_carrier G ==> i IN k
+                   then group_product G (<<=) k f
+                   else group_mul G (f i) (group_product G (<<=) k f))`,
+  REPEAT STRIP_TAC THEN ASM_SIMP_TAC[group_product; ITERATO_CLAUSES] THEN
+  ASM_CASES_TAC `(i:K) IN k` THEN ASM_REWRITE_TAC[] THEN
+  ASM_CASES_TAC `(f:K->A) i = group_id G` THEN ASM_REWRITE_TAC[] THEN
+  SIMP_TAC[GROUP_MUL_LID; GSYM group_product; GROUP_PRODUCT; GROUP_ID]);;
+
+let GROUP_PRODUCT_CLAUSES_EXISTS = prove
+ (`!G (<<=) (f:K->A).
+      group_product G (<<=) {} f = group_id G /\
+      (!k. FINITE {i | i IN k /\ f i IN group_carrier G DIFF {group_id G}} /\
+           ~({i | i IN k /\ f i IN group_carrier G DIFF {group_id G}} = {})
+           ==> ?i. i IN k /\
+                   f i IN group_carrier G DIFF {group_id G} /\
+                   group_product G (<<=) k f =
+                   group_mul G (f i) (group_product G (<<=) (k DELETE i) f))`,
+  REWRITE_TAC[group_product] THEN
+  MATCH_ACCEPT_TAC ITERATO_CLAUSES_EXISTS);;
+
+let GROUP_SUM_CLAUSES_EXISTS = prove
+ (`!G (f:K->A).
+      group_sum G {} f = group_id G /\
+      (!k. FINITE {i | i IN k /\ f i IN group_carrier G DIFF {group_id G}} /\
+           ~({i | i IN k /\ f i IN group_carrier G DIFF {group_id G}} = {})
+           ==> ?i. i IN k /\
+                   f i IN group_carrier G DIFF {group_id G} /\
+                   group_sum G k f =
+                   group_mul G (f i) (group_sum G (k DELETE i) f))`,
+  REWRITE_TAC[group_sum] THEN MATCH_ACCEPT_TAC GROUP_PRODUCT_CLAUSES_EXISTS);;
+
+let GROUP_COMMUTES_PRODUCT = prove
+ (`!G (<<=) k (f:K->A) z.
+        (!i. i IN k /\ f i IN group_carrier G /\ ~(f i = group_id G)
+             ==> group_mul G (f i) z = group_mul G z (f i)) /\
+        z IN group_carrier G
+        ==> group_mul G (group_product G (<<=) k f) z =
+            group_mul G z (group_product G (<<=) k f)`,
+  REPEAT STRIP_TAC THEN
+  MATCH_MP_TAC(REWRITE_RULE[]
+   (ISPEC `\x:A. group_mul G x z = group_mul G z x` GROUP_PRODUCT_CLOSED)) THEN
+  ASM_SIMP_TAC[GROUP_MUL_LID; GROUP_MUL_RID] THEN
+  ASM_MESON_TAC[GROUP_COMMUTES_MUL]);;
+
+let GROUP_COMMUTES_SUM = prove
+ (`!G k (f:K->A) z.
+        (!i. i IN k /\ f i IN group_carrier G /\ ~(f i = group_id G)
+             ==> group_mul G (f i) z = group_mul G z (f i)) /\
+        z IN group_carrier G
+        ==> group_mul G (group_sum G k f) z = group_mul G z (group_sum G k f)`,
+  REWRITE_TAC[group_sum; GROUP_COMMUTES_PRODUCT]);;
+
+let GROUP_PRODUCT_SING = prove
+ (`!G (<<=) i (f:K->A).
+        group_product G (<<=) {i} f =
+        if f i IN group_carrier G then f i else group_id G`,
+  REPEAT GEN_TAC THEN
+  SIMP_TAC[GROUP_PRODUCT_CLAUSES; NOT_IN_EMPTY; EMPTY_GSPEC; FINITE_EMPTY] THEN
+  SIMP_TAC[COND_SWAP; GROUP_MUL_RID]);;
+
+let GROUP_SUM_SING = prove
+ (`!G i (f:K->A).
+        group_sum G {i} f =
+        if f i IN group_carrier G then f i else group_id G`,
+  REWRITE_TAC[group_sum; GROUP_PRODUCT_SING]);;
+
+let GROUP_PRODUCT_UNION = prove
+ (`!G (<<=) (f:K->A) s t.
+        woset(<<=) /\ fld(<<=) = (:K) /\
+        (FINITE {i | i IN s /\ f i IN group_carrier G DIFF {group_id G}} <=>
+         FINITE {i | i IN t /\ f i IN group_carrier G DIFF {group_id G}}) /\
+        (!x y. x IN s /\ y IN t ==> x <<= y /\ ~(x = y))
+        ==> group_product G (<<=) (s UNION t) f =
+            group_mul G (group_product G (<<=) s f)
+                        (group_product G (<<=) t f)`,
+  REPEAT STRIP_TAC THEN ONCE_REWRITE_TAC[GROUP_PRODUCT_EXPAND_CASES] THEN
+  REWRITE_TAC[SET_RULE
+   `{x | x IN s UNION t /\ P x} =
+    {x | x IN s /\ P x} UNION {x | x IN t /\ P x}`] THEN
+  REWRITE_TAC[FINITE_UNION] THEN ASM_CASES_TAC
+  `FINITE {i | i IN t /\ (f:K->A) i IN group_carrier G DIFF {group_id G}}` THEN
+  ASM_SIMP_TAC[GROUP_MUL_LID; GROUP_ID] THEN
+  SUBGOAL_THEN
+   `(!i. i IN {i | i IN s /\ (f:K->A) i IN group_carrier G DIFF {group_id G}}
+         ==> f i IN group_carrier G /\ ~(f i = group_id G)) /\
+    (!i. i IN {i | i IN t /\ (f:K->A) i IN group_carrier G DIFF {group_id G}}
+         ==> f i IN group_carrier G /\ ~(f i = group_id G))`
+  MP_TAC THENL [ASM SET_TAC[]; ALL_TAC] THEN
+  SUBGOAL_THEN
+   `!x y. x IN {i | i IN s /\ f i IN group_carrier G DIFF {group_id G}} /\
+          y IN {i | i IN t /\ (f:K->A) i IN group_carrier G DIFF {group_id G}}
+          ==> x <<= y /\ ~(x = y)`
+  MP_TAC THENL [ASM SET_TAC[]; ALL_TAC] THEN
+  FIRST_X_ASSUM(MP_TAC o MATCH_MP (TAUT `(p <=> q) ==> (q ==> q /\ p)`)) THEN
+  ANTS_TAC THENL [ASM_REWRITE_TAC[]; ALL_TAC] THEN
+  MAP_EVERY UNDISCH_TAC [`fld(<<=) = (:K)`; `woset((<<=):K->K->bool)`] THEN
+  POP_ASSUM_LIST(K ALL_TAC) THEN DISCH_TAC THEN DISCH_TAC THEN
+  SPEC_TAC(`{i | i IN s /\ (f:K->A) i IN group_carrier G DIFF {group_id G}}`,
+           `s:K->bool`) THEN
+  SPEC_TAC(`{i | i IN t /\ (f:K->A) i IN group_carrier G DIFF {group_id G}}`,
+           `t:K->bool`) THEN
+  REWRITE_TAC[IMP_CONJ; RIGHT_FORALL_IMP_THM] THEN
+  X_GEN_TAC `t:K->bool` THEN DISCH_TAC THEN ASM_CASES_TAC
+   `!i. i IN t ==> (f:K->A) i IN group_carrier G /\ ~(f i = group_id G)` THEN
+  ASM_REWRITE_TAC[GSYM CONJ_ASSOC; IMP_IMP] THEN
+  ONCE_REWRITE_TAC[IMP_CONJ] THEN MATCH_MP_TAC(MESON[]
+   `(!n s. FINITE s /\ CARD s = n ==> P s) ==> !s. FINITE s ==> P s`) THEN
+  MATCH_MP_TAC num_WF THEN X_GEN_TAC `n:num` THEN DISCH_TAC THEN
+  X_GEN_TAC `s:K->bool` THEN
+  ASM_CASES_TAC `s:K->bool = {}` THEN
+  ASM_REWRITE_TAC[UNION_EMPTY; GROUP_PRODUCT_CLAUSES_EXISTS] THEN
+  SIMP_TAC[GROUP_MUL_LID; GROUP_PRODUCT] THEN REPEAT STRIP_TAC THEN
+  FIRST_ASSUM(MP_TAC o SPEC `s:K->bool` o last o CONJUNCTS o
+        GEN_REWRITE_RULE I [woset]) THEN
+  ASM_REWRITE_TAC[SUBSET_UNIV; LEFT_IMP_EXISTS_THM] THEN
+  X_GEN_TAC `i:K` THEN STRIP_TAC THEN
+  MP_TAC(ISPECL [`G:A group`; `(<<=):K->K->bool`; `f:K->A`]
+        GROUP_PRODUCT_CLAUSES) THEN
+  DISCH_THEN(MP_TAC o SPEC `i:K` o CONJUNCT2) THEN DISCH_THEN(fun th ->
+    MP_TAC(SPEC `s DELETE (i:K)` th) THEN
+    MP_TAC(SPEC `(s DELETE (i:K)) UNION t` th)) THEN
+  ASM_SIMP_TAC[FINITE_DELETE; FINITE_UNION; FINITE_RESTRICT;
+    IN_DELETE; IN_UNION;
+    SET_RULE `i IN s ==> i INSERT (s DELETE i) = s`;
+    SET_RULE `i IN s ==> i INSERT (s DELETE i UNION t) = s UNION t`] THEN
+  FIRST_X_ASSUM(MP_TAC o GEN_REWRITE_RULE I [woset]) THEN
+  ASM_REWRITE_TAC[IN_UNIV] THEN STRIP_TAC THEN
+  ANTS_TAC THENL [ASM_MESON_TAC[]; DISCH_THEN SUBST1_TAC] THEN
+  ANTS_TAC THENL [ASM_MESON_TAC[]; DISCH_THEN SUBST1_TAC] THEN
+  COND_CASES_TAC THENL [ASM_MESON_TAC[]; ALL_TAC] THEN
+  FIRST_X_ASSUM(MP_TAC o SPEC `n - 1`) THEN
+  REWRITE_TAC[ARITH_RULE `n - 1 < n <=> ~(n = 0)`] THEN
+  ANTS_TAC THENL [ASM_MESON_TAC[CARD_EQ_0]; ALL_TAC] THEN
+  DISCH_THEN(MP_TAC o SPEC `s DELETE (i:K)`) THEN
+  ASM_SIMP_TAC[FINITE_DELETE; CARD_DELETE; IN_DELETE] THEN
+  ASM_SIMP_TAC[GROUP_MUL_ASSOC; GROUP_MUL; GROUP_PRODUCT]);;
+
+let GROUP_PRODUCT_CLAUSES_LEFT = prove
+ (`!G (f:num->A) m n.
+        group_product G (<=) (m..n) f =
+        if m <= n then
+           if f m IN group_carrier G
+           then group_mul G (f m) (group_product G (<=) (m+1..n) f)
+           else group_product G (<=) (m+1..n) f
+         else group_id G`,
+  REPEAT GEN_TAC THEN COND_CASES_TAC THENL
+   [ASM_SIMP_TAC[GSYM NUMSEG_LREC];
+    ASM_SIMP_TAC[EMPTY_NUMSEG; GSYM NOT_LE; GROUP_PRODUCT_CLAUSES]] THEN
+  ONCE_REWRITE_TAC[SET_RULE `a INSERT s = {a} UNION s`] THEN
+  W(MP_TAC o PART_MATCH (lhand o rand) GROUP_PRODUCT_UNION o lhand o snd) THEN
+  SIMP_TAC[WOSET_num; FLD_num; FINITE_RESTRICT; FINITE_SING; FINITE_NUMSEG;
+           IN_NUMSEG; IN_SING] THEN
+  ANTS_TAC THENL [ARITH_TAC; DISCH_THEN SUBST1_TAC] THEN
+  REWRITE_TAC[GROUP_PRODUCT_SING] THEN
+  COND_CASES_TAC THEN ASM_SIMP_TAC[GROUP_MUL_LID; GROUP_PRODUCT]);;
+
+let GROUP_PRODUCT_CLAUSES_RIGHT = prove
+ (`!G (f:num->A) m n.
+        group_product G (<=) (m..n) f =
+        if m <= n then
+           if f n IN group_carrier G
+           then if n = 0 then f 0
+                else group_mul G (group_product G (<=) (m..n-1) f) (f n)
+           else group_product G (<=) (m..n-1) f
+         else group_id G`,
+  REPEAT GEN_TAC THEN ASM_CASES_TAC `n = 0` THENL
+   [ASM_SIMP_TAC[CONJUNCT1 LE; SUB_0; NUMSEG_CLAUSES] THEN
+    ASM_CASES_TAC `m = 0` THEN ASM_SIMP_TAC[GROUP_PRODUCT_SING] THEN
+    REWRITE_TAC[GROUP_PRODUCT_CLAUSES];
+    ASM_REWRITE_TAC[]] THEN
+  COND_CASES_TAC THEN ASM_REWRITE_TAC[] THENL
+   [ASM_SIMP_TAC[GSYM NUMSEG_RREC];
+    ASM_SIMP_TAC[EMPTY_NUMSEG; GSYM NOT_LE; GROUP_PRODUCT_CLAUSES]] THEN
+  ONCE_REWRITE_TAC[SET_RULE `a INSERT s = s UNION {a}`] THEN
+  W(MP_TAC o PART_MATCH (lhand o rand) GROUP_PRODUCT_UNION o lhand o snd) THEN
+  SIMP_TAC[WOSET_num; FLD_num; FINITE_RESTRICT; FINITE_SING; FINITE_NUMSEG;
+           IN_NUMSEG; IN_SING] THEN
+  ANTS_TAC THENL [ASM_ARITH_TAC; DISCH_THEN SUBST1_TAC] THEN
+  REWRITE_TAC[GROUP_PRODUCT_SING] THEN
+  COND_CASES_TAC THEN ASM_SIMP_TAC[GROUP_MUL_RID; GROUP_PRODUCT]);;
+
+let GROUP_PRODUCT_CLAUSES_NUMSEG = prove
+ (`(!G m f:num->A.
+        group_product G (<=) (m..0) f =
+        if m = 0 /\ f 0 IN group_carrier G then f 0 else group_id G) /\
+   (!G m n f:num->A.
+        group_product G (<=) (m..SUC n) f =
+        if m <= SUC n /\ f(SUC n) IN group_carrier G
+        then group_mul G (group_product G (<=) (m..n) f) (f(SUC n))
+        else group_product G (<=) (m..n) f)`,
+  REPEAT STRIP_TAC THEN
+  GEN_REWRITE_TAC LAND_CONV [GROUP_PRODUCT_CLAUSES_RIGHT] THEN
+  SIMP_TAC[CONJUNCT1 LE; NOT_SUC; SUC_SUB1; SUB_0; NUMSEG_SING;
+           GROUP_PRODUCT_SING]
+  THENL [MESON_TAC[]; ALL_TAC] THEN
+  ASM_CASES_TAC `m <= SUC n` THEN ASM_REWRITE_TAC[] THEN
+  ASM_SIMP_TAC[EMPTY_NUMSEG; ARITH_RULE `~(m <= SUC n) ==> n < m`] THEN
+  REWRITE_TAC[GROUP_PRODUCT_CLAUSES]);;
+
+let GROUP_PRODUCT_CLAUSES_COMMUTING = prove
+ (`!G (<<=) i k (f:K->A).
+        woset(<<=) /\ fld(<<=) = (:K) /\
+        FINITE {j | j IN k /\ f j IN group_carrier G DIFF {group_id G}} /\
+        (!j. j IN k /\ j <<= i /\ ~(j = i) /\
+             f i IN group_carrier G /\ f j IN group_carrier G
+             ==> group_mul G (f i) (f j) = group_mul G (f j) (f i))
+        ==> group_product G (<<=) (i INSERT k) f =
+                if f i IN group_carrier G ==> i IN k
+                then group_product G (<<=) k f
+                else group_mul G (f i) (group_product G (<<=) k f)`,
+  let tac pfn =
+    W(MP_TAC o PART_MATCH (lhand o rand) GROUP_PRODUCT_UNION o pfn o snd) THEN
+    ASM_REWRITE_TAC[] THEN ANTS_TAC THENL
+     [REWRITE_TAC[CONJ_ASSOC] THEN CONJ_TAC THENL
+       [MATCH_MP_TAC(TAUT `p /\ q ==> (p <=> q)`) THEN CONJ_TAC THEN
+        FIRST_X_ASSUM(MATCH_MP_TAC o MATCH_MP
+         (MESON[FINITE_INSERT; FINITE_SUBSET]
+          `FINITE s ==> !i. t SUBSET i INSERT s ==> FINITE t`)) THEN
+        EXISTS_TAC `i:K` THEN SET_TAC[];
+        FIRST_X_ASSUM(MP_TAC o GEN_REWRITE_RULE I [woset]) THEN
+        ASM_REWRITE_TAC[IN_UNIV] THEN ASM SET_TAC[];];
+      DISCH_THEN SUBST1_TAC] in
+  REPEAT STRIP_TAC THEN COND_CASES_TAC THENL
+   [ONCE_REWRITE_TAC[GSYM GROUP_PRODUCT_RESTRICT] THEN
+    ONCE_REWRITE_TAC[GSYM GROUP_PRODUCT_SUPPORT] THEN
+    AP_THM_TAC THEN AP_TERM_TAC THEN ASM SET_TAC[];
+    FIRST_X_ASSUM(STRIP_ASSUME_TAC o GEN_REWRITE_RULE I [NOT_IMP])] THEN
+  SUBGOAL_THEN
+   `k = {j:K | j IN k /\ j <<= i /\ ~(j = i)} UNION
+        {j | j IN k /\ i <<= j /\ ~(j = i)}`
+  SUBST1_TAC THENL
+   [FIRST_X_ASSUM(MP_TAC o GEN_REWRITE_RULE I [woset]) THEN
+    ASM_REWRITE_TAC[IN_UNIV] THEN ASM SET_TAC[];
+    ONCE_REWRITE_TAC[SET_RULE
+     `i INSERT (l UNION r) = (i INSERT l) UNION r`]] THEN
+  tac lhand THEN
+  ONCE_REWRITE_TAC[SET_RULE `i INSERT s = s UNION {i}`] THEN
+  tac (lhand o lhand) THEN
+  tac (rand o rand) THEN
+   ASM_SIMP_TAC[GROUP_MUL_ASSOC; GROUP_PRODUCT] THEN
+  AP_THM_TAC THEN AP_TERM_TAC THEN ASM_REWRITE_TAC[GROUP_PRODUCT_SING] THEN
+  MATCH_MP_TAC GROUP_COMMUTES_PRODUCT THEN ASM SET_TAC[]);;
+
+let ABELIAN_GROUP_PRODUCT_CLAUSES = prove
+ (`!G (<<=) i k (f:K->A).
+        woset(<<=) /\ fld(<<=) = (:K) /\
+        abelian_group G /\
+        FINITE {j | j IN k /\ f j IN group_carrier G DIFF {group_id G}}
+        ==> group_product G (<<=) (i INSERT k) f =
+                if f i IN group_carrier G ==> i IN k
+                then group_product G (<<=) k f
+                else group_mul G (f i) (group_product G (<<=) k f)`,
+  REPEAT STRIP_TAC THEN MATCH_MP_TAC GROUP_PRODUCT_CLAUSES_COMMUTING THEN
+  ASM_REWRITE_TAC[] THEN ASM_MESON_TAC[abelian_group]);;
+
+let GROUP_SUM_CLAUSES_COMMUTING = prove
+ (`!G i k (f:K->A).
+        FINITE {j | j IN k /\ f j IN group_carrier G DIFF {group_id G}} /\
+        (!j. j IN k /\ ~(j = i) /\
+             f i IN group_carrier G /\ f j IN group_carrier G
+             ==> group_mul G (f i) (f j) = group_mul G (f j) (f i))
+        ==> group_sum G (i INSERT k) f =
+                if f i IN group_carrier G ==> i IN k
+                then group_sum G k f
+                else group_mul G (f i) (group_sum G k f)`,
+  REPEAT STRIP_TAC THEN REWRITE_TAC[group_sum] THEN
+  MATCH_MP_TAC GROUP_PRODUCT_CLAUSES_COMMUTING THEN ASM_SIMP_TAC[] THEN
+  CONV_TAC SELECT_CONV THEN REWRITE_TAC[WO]);;
+
+let ABELIAN_GROUP_SUM_CLAUSES = prove
+ (`!G i k (f:K->A).
+        abelian_group G /\
+        FINITE {j | j IN k /\ f j IN group_carrier G DIFF {group_id G}}
+        ==> group_sum G (i INSERT k) f =
+                if f i IN group_carrier G ==> i IN k
+                then group_sum G k f
+                else group_mul G (f i) (group_sum G k f)`,
+  REPEAT STRIP_TAC THEN MATCH_MP_TAC GROUP_SUM_CLAUSES_COMMUTING THEN
+  ASM_MESON_TAC[abelian_group]);;
+
+let GROUP_PRODUCT_MUL = prove
+ (`!G (<<=) k f (g:K->A).
+      woset(<<=) /\ fld(<<=) = (:K) /\
+      FINITE {i | i IN k /\ ~(f i = group_id G)} /\
+      FINITE {i | i IN k /\ ~(g i = group_id G)} /\
+      (!i. i IN k ==> f i IN group_carrier G /\ g i IN group_carrier G) /\
+      pairwise (\i j. group_mul G (f i) (g j) = group_mul G (g j) (f i)) k
+      ==> group_product G (<<=) k (\i. group_mul G (f i) (g i)) =
+          group_mul G (group_product G (<<=) k f) (group_product G (<<=) k g)`,
+  GEN_REWRITE_TAC (funpow 2 BINDER_CONV) [SWAP_FORALL_THM] THEN
+  GEN_REWRITE_TAC (funpow 3 BINDER_CONV) [SWAP_FORALL_THM] THEN
+  REWRITE_TAC[RIGHT_FORALL_IMP_THM; IMP_CONJ] THEN
+  REPEAT GEN_TAC THEN DISCH_TAC THEN DISCH_TAC THEN GEN_TAC THEN GEN_TAC THEN
+  ONCE_REWRITE_TAC[IMP_IMP] THEN REWRITE_TAC[GSYM FINITE_UNION] THEN
+  X_GEN_TAC `s:K->bool` THEN
+  W(fun (asl,w) -> ABBREV_TAC(mk_eq(`t:K->bool`,rand(lhand w)))) THEN
+  REPEAT STRIP_TAC THEN
+  SUBGOAL_THEN
+   `group_product G (<<=) t (\i. group_mul G (f i) (g i)) =
+    group_mul G (group_product G (<<=) t (f:K->A)) (group_product G (<<=) t g)`
+  MP_TAC THENL
+   [SUBGOAL_THEN
+     `!i. i IN t ==> (f:K->A) i IN group_carrier G /\ g i IN group_carrier G`
+    MP_TAC THENL [ASM SET_TAC[]; ALL_TAC] THEN
+    FIRST_X_ASSUM(MP_TAC o SPEC `t:K->bool` o MATCH_MP
+     (REWRITE_RULE[IMP_CONJ] PAIRWISE_MONO)) THEN
+    ANTS_TAC THENL [ASM SET_TAC[]; UNDISCH_TAC `FINITE(t:K->bool)`] THEN
+    FIRST_X_ASSUM(K ALL_TAC o SYM) THEN
+    FIRST_X_ASSUM(K ALL_TAC o check (is_forall o concl));
+    MATCH_MP_TAC EQ_IMP THEN BINOP_TAC THENL
+     [ALL_TAC; BINOP_TAC] THEN
+    ONCE_REWRITE_TAC[GSYM GROUP_PRODUCT_RESTRICT] THEN
+    ONCE_REWRITE_TAC[GSYM GROUP_PRODUCT_SUPPORT] THEN
+    AP_THM_TAC THEN AP_TERM_TAC THEN
+    MP_TAC(ISPEC `G:A group` GROUP_MUL_LID) THEN
+    MP_TAC(ISPEC `G:A group` GROUP_MUL_RID) THEN ASM SET_TAC[]] THEN
+  SPEC_TAC(`t:K->bool`,`s:K->bool`) THEN MATCH_MP_TAC(MESON[]
+   `(!n s. FINITE s /\ CARD s = n ==> P s)
+    ==> !s. FINITE s ==> P s`) THEN
+  MATCH_MP_TAC num_WF THEN X_GEN_TAC `n:num` THEN DISCH_TAC THEN
+  X_GEN_TAC `s:K->bool` THEN ONCE_REWRITE_TAC[IMP_CONJ] THEN
+  ASM_CASES_TAC `n = 0` THENL
+   [ASM_SIMP_TAC[CARD_EQ_0] THEN
+    REWRITE_TAC[GROUP_PRODUCT_CLAUSES] THEN SIMP_TAC[GROUP_MUL_LID; GROUP_ID];
+    REPEAT DISCH_TAC THEN
+    FIRST_ASSUM(MP_TAC o MATCH_MP (MESON[CARD_EQ_0]
+     `CARD s = n ==> FINITE s /\ ~(n = 0) ==> ~(s = {})`)) THEN
+    ASM_REWRITE_TAC[]] THEN
+  FIRST_ASSUM(MP_TAC o last o CONJUNCTS o GEN_REWRITE_RULE I [woset]) THEN
+  ASM_REWRITE_TAC[IMP_IMP; SUBSET_UNIV] THEN
+  DISCH_THEN(MP_TAC o MATCH_MP (MESON[]
+   `(!s. ~(s = {}) ==> P s) /\ ~(t = {}) ==> P t`)) THEN
+  DISCH_THEN(X_CHOOSE_THEN `i:K` STRIP_ASSUME_TAC) THEN
+  SUBGOAL_THEN `s = {i:K} UNION (s DELETE i)` SUBST1_TAC THENL
+   [ASM SET_TAC[]; ALL_TAC] THEN
+  W(MP_TAC o PART_MATCH (lhand o rand) GROUP_PRODUCT_UNION o lhand o snd) THEN
+  ASM_SIMP_TAC[FINITE_DELETE; FINITE_RESTRICT; FINITE_SING] THEN
+  ANTS_TAC THENL [ASM SET_TAC[]; DISCH_THEN SUBST1_TAC] THEN
+  W(MP_TAC o PART_MATCH (lhand o rand) GROUP_PRODUCT_UNION o
+    lhand o rand o snd) THEN
+  ASM_SIMP_TAC[FINITE_DELETE; FINITE_RESTRICT; FINITE_SING] THEN
+  ANTS_TAC THENL [ASM SET_TAC[]; DISCH_THEN SUBST1_TAC] THEN
+  W(MP_TAC o PART_MATCH (lhand o rand) GROUP_PRODUCT_UNION o
+    rand o rand o snd) THEN
+  ASM_SIMP_TAC[FINITE_DELETE; FINITE_RESTRICT; FINITE_SING] THEN
+  ANTS_TAC THENL [ASM SET_TAC[]; DISCH_THEN SUBST1_TAC] THEN
+  REWRITE_TAC[GROUP_PRODUCT_SING] THEN
+  FIRST_X_ASSUM(MP_TAC o SPEC `n - 1`) THEN
+  REWRITE_TAC[ARITH_RULE `n - 1 < n <=> ~(n = 0)`] THEN
+  ANTS_TAC THENL [ASM_MESON_TAC[CARD_EQ_0]; ALL_TAC] THEN
+  DISCH_THEN(MP_TAC o SPEC `s DELETE (i:K)`) THEN
+  ASM_SIMP_TAC[FINITE_DELETE; CARD_DELETE; IN_DELETE] THEN ANTS_TAC THENL
+   [FIRST_X_ASSUM(MATCH_MP_TAC o MATCH_MP
+     (REWRITE_RULE[IMP_CONJ] PAIRWISE_MONO)) THEN
+    SET_TAC[];
+    DISCH_THEN SUBST1_TAC] THEN
+  ASM_SIMP_TAC[GSYM GROUP_MUL_ASSOC; GROUP_MUL; GROUP_PRODUCT] THEN
+  AP_TERM_TAC THEN
+  ASM_SIMP_TAC[GROUP_MUL_ASSOC; GROUP_MUL; GROUP_PRODUCT] THEN
+  AP_THM_TAC THEN AP_TERM_TAC THEN
+  CONV_TAC SYM_CONV THEN MATCH_MP_TAC GROUP_COMMUTES_PRODUCT THEN
+  FIRST_X_ASSUM(MP_TAC o GEN_REWRITE_RULE I [pairwise]) THEN ASM SET_TAC[]);;
+
+let GROUP_SUM_MUL = prove
+ (`!G k f (g:K->A).
+        FINITE {i | i IN k /\ ~(f i = group_id G)} /\
+        FINITE {i | i IN k /\ ~(g i = group_id G)} /\
+        (!i. i IN k ==> f i IN group_carrier G /\ g i IN group_carrier G) /\
+        pairwise (\i j. group_mul G (f i) (g j) = group_mul G (g j) (f i)) k
+        ==> group_sum G k (\i. group_mul G (f i) (g i)) =
+            group_mul G (group_sum G k f) (group_sum G k g)`,
+  REPEAT STRIP_TAC THEN REWRITE_TAC[group_sum] THEN
+  MATCH_MP_TAC GROUP_PRODUCT_MUL THEN ASM_REWRITE_TAC[] THEN
+  CONV_TAC SELECT_CONV THEN REWRITE_TAC[WO]);;
 
 (* ------------------------------------------------------------------------- *)
 (* Congugation.                                                              *)
